---
layout: default
title: Observables - likelihood_eeww.yaml
---

# List of all observables included in likelihood_eeww.yaml

{: class="table"}
| Symbol | Name | Arguments | SM Prediction | 
|--------|------|-----------|---------------|
| $R(e^+e^- \to W^+W^-)$ | `R(ee->WW)` | E = 182.7 |1.0 | 
| $R(e^+e^- \to W^+W^-)$ | `R(ee->WW)` | E = 188.6 |1.0 | 
| $R(e^+e^- \to W^+W^-)$ | `R(ee->WW)` | E = 191.6 |1.0 | 
| $R(e^+e^- \to W^+W^-)$ | `R(ee->WW)` | E = 195.5 |1.0 | 
| $R(e^+e^- \to W^+W^-)$ | `R(ee->WW)` | E = 199.5 |1.0 | 
| $R(e^+e^- \to W^+W^-)$ | `R(ee->WW)` | E = 201.6 |1.0 | 
| $R(e^+e^- \to W^+W^-)$ | `R(ee->WW)` | E = 204.9 |1.0 | 
| $R(e^+e^- \to W^+W^-)$ | `R(ee->WW)` | E = 206.6 |1.0 | 
| $\left\langle\frac{dR}{d\theta}\right\rangle(e^+e^- \to W^+W^-)$ | `<dR/dtheta>(ee->WW)` | E = 182.66, thetamin = -1.0, thetamax = -0.8 |0.702 | 
| $\left\langle\frac{dR}{d\theta}\right\rangle(e^+e^- \to W^+W^-)$ | `<dR/dtheta>(ee->WW)` | E = 182.66, thetamin = -0.8, thetamax = -0.6 |0.841 | 
| $\left\langle\frac{dR}{d\theta}\right\rangle(e^+e^- \to W^+W^-)$ | `<dR/dtheta>(ee->WW)` | E = 182.66, thetamin = -0.6, thetamax = -0.4 |1.011 | 
| $\left\langle\frac{dR}{d\theta}\right\rangle(e^+e^- \to W^+W^-)$ | `<dR/dtheta>(ee->WW)` | E = 182.66, thetamin = -0.4, thetamax = -0.2 |1.181 | 
| $\left\langle\frac{dR}{d\theta}\right\rangle(e^+e^- \to W^+W^-)$ | `<dR/dtheta>(ee->WW)` | E = 182.66, thetamin = -0.2, thetamax = 0.0 |1.402 | 
| $\left\langle\frac{dR}{d\theta}\right\rangle(e^+e^- \to W^+W^-)$ | `<dR/dtheta>(ee->WW)` | E = 182.66, thetamin = 0.0, thetamax = 0.2 |1.731 | 
| $\left\langle\frac{dR}{d\theta}\right\rangle(e^+e^- \to W^+W^-)$ | `<dR/dtheta>(ee->WW)` | E = 182.66, thetamin = 0.2, thetamax = 0.4 |2.189 | 
| $\left\langle\frac{dR}{d\theta}\right\rangle(e^+e^- \to W^+W^-)$ | `<dR/dtheta>(ee->WW)` | E = 182.66, thetamin = 0.4, thetamax = 0.6 |2.822 | 
| $\left\langle\frac{dR}{d\theta}\right\rangle(e^+e^- \to W^+W^-)$ | `<dR/dtheta>(ee->WW)` | E = 182.66, thetamin = 0.6, thetamax = 0.8 |3.806 | 
| $\left\langle\frac{dR}{d\theta}\right\rangle(e^+e^- \to W^+W^-)$ | `<dR/dtheta>(ee->WW)` | E = 182.66, thetamin = 0.8, thetamax = 1.0 |5.434 | 
| $\left\langle\frac{dR}{d\theta}\right\rangle(e^+e^- \to W^+W^-)$ | `<dR/dtheta>(ee->WW)` | E = 189.09, thetamin = -1.0, thetamax = -0.8 |0.661 | 
| $\left\langle\frac{dR}{d\theta}\right\rangle(e^+e^- \to W^+W^-)$ | `<dR/dtheta>(ee->WW)` | E = 189.09, thetamin = -0.8, thetamax = -0.6 |0.781 | 
| $\left\langle\frac{dR}{d\theta}\right\rangle(e^+e^- \to W^+W^-)$ | `<dR/dtheta>(ee->WW)` | E = 189.09, thetamin = -0.6, thetamax = -0.4 |0.928 | 
| $\left\langle\frac{dR}{d\theta}\right\rangle(e^+e^- \to W^+W^-)$ | `<dR/dtheta>(ee->WW)` | E = 189.09, thetamin = -0.4, thetamax = -0.2 |1.137 | 
| $\left\langle\frac{dR}{d\theta}\right\rangle(e^+e^- \to W^+W^-)$ | `<dR/dtheta>(ee->WW)` | E = 189.09, thetamin = -0.2, thetamax = 0.0 |1.403 | 
| $\left\langle\frac{dR}{d\theta}\right\rangle(e^+e^- \to W^+W^-)$ | `<dR/dtheta>(ee->WW)` | E = 189.09, thetamin = 0.0, thetamax = 0.2 |1.715 | 
| $\left\langle\frac{dR}{d\theta}\right\rangle(e^+e^- \to W^+W^-)$ | `<dR/dtheta>(ee->WW)` | E = 189.09, thetamin = 0.2, thetamax = 0.4 |2.187 | 
| $\left\langle\frac{dR}{d\theta}\right\rangle(e^+e^- \to W^+W^-)$ | `<dR/dtheta>(ee->WW)` | E = 189.09, thetamin = 0.4, thetamax = 0.6 |2.946 | 
| $\left\langle\frac{dR}{d\theta}\right\rangle(e^+e^- \to W^+W^-)$ | `<dR/dtheta>(ee->WW)` | E = 189.09, thetamin = 0.6, thetamax = 0.8 |4.122 | 
| $\left\langle\frac{dR}{d\theta}\right\rangle(e^+e^- \to W^+W^-)$ | `<dR/dtheta>(ee->WW)` | E = 189.09, thetamin = 0.8, thetamax = 1.0 |6.253 | 
| $\left\langle\frac{dR}{d\theta}\right\rangle(e^+e^- \to W^+W^-)$ | `<dR/dtheta>(ee->WW)` | E = 198.38, thetamin = -1.0, thetamax = -0.8 |0.542 | 
| $\left\langle\frac{dR}{d\theta}\right\rangle(e^+e^- \to W^+W^-)$ | `<dR/dtheta>(ee->WW)` | E = 198.38, thetamin = -0.8, thetamax = -0.6 |0.664 | 
| $\left\langle\frac{dR}{d\theta}\right\rangle(e^+e^- \to W^+W^-)$ | `<dR/dtheta>(ee->WW)` | E = 198.38, thetamin = -0.6, thetamax = -0.4 |0.835 | 
| $\left\langle\frac{dR}{d\theta}\right\rangle(e^+e^- \to W^+W^-)$ | `<dR/dtheta>(ee->WW)` | E = 198.38, thetamin = -0.4, thetamax = -0.2 |1.021 | 
| $\left\langle\frac{dR}{d\theta}\right\rangle(e^+e^- \to W^+W^-)$ | `<dR/dtheta>(ee->WW)` | E = 198.38, thetamin = -0.2, thetamax = 0.0 |1.265 | 
| $\left\langle\frac{dR}{d\theta}\right\rangle(e^+e^- \to W^+W^-)$ | `<dR/dtheta>(ee->WW)` | E = 198.38, thetamin = 0.0, thetamax = 0.2 |1.666 | 
| $\left\langle\frac{dR}{d\theta}\right\rangle(e^+e^- \to W^+W^-)$ | `<dR/dtheta>(ee->WW)` | E = 198.38, thetamin = 0.2, thetamax = 0.4 |2.161 | 
| $\left\langle\frac{dR}{d\theta}\right\rangle(e^+e^- \to W^+W^-)$ | `<dR/dtheta>(ee->WW)` | E = 198.38, thetamin = 0.4, thetamax = 0.6 |3.003 | 
| $\left\langle\frac{dR}{d\theta}\right\rangle(e^+e^- \to W^+W^-)$ | `<dR/dtheta>(ee->WW)` | E = 198.38, thetamin = 0.6, thetamax = 0.8 |4.428 | 
| $\left\langle\frac{dR}{d\theta}\right\rangle(e^+e^- \to W^+W^-)$ | `<dR/dtheta>(ee->WW)` | E = 198.38, thetamin = 0.8, thetamax = 1.0 |7.236 | 
| $\left\langle\frac{dR}{d\theta}\right\rangle(e^+e^- \to W^+W^-)$ | `<dR/dtheta>(ee->WW)` | E = 205.92, thetamin = -1.0, thetamax = -0.8 |0.532 | 
| $\left\langle\frac{dR}{d\theta}\right\rangle(e^+e^- \to W^+W^-)$ | `<dR/dtheta>(ee->WW)` | E = 205.92, thetamin = -0.8, thetamax = -0.6 |0.642 | 
| $\left\langle\frac{dR}{d\theta}\right\rangle(e^+e^- \to W^+W^-)$ | `<dR/dtheta>(ee->WW)` | E = 205.92, thetamin = -0.6, thetamax = -0.4 |0.77 | 
| $\left\langle\frac{dR}{d\theta}\right\rangle(e^+e^- \to W^+W^-)$ | `<dR/dtheta>(ee->WW)` | E = 205.92, thetamin = -0.4, thetamax = -0.2 |0.972 | 
| $\left\langle\frac{dR}{d\theta}\right\rangle(e^+e^- \to W^+W^-)$ | `<dR/dtheta>(ee->WW)` | E = 205.92, thetamin = -0.2, thetamax = 0.0 |1.231 | 
| $\left\langle\frac{dR}{d\theta}\right\rangle(e^+e^- \to W^+W^-)$ | `<dR/dtheta>(ee->WW)` | E = 205.92, thetamin = 0.0, thetamax = 0.2 |1.561 | 
| $\left\langle\frac{dR}{d\theta}\right\rangle(e^+e^- \to W^+W^-)$ | `<dR/dtheta>(ee->WW)` | E = 205.92, thetamin = 0.2, thetamax = 0.4 |2.056 | 
| $\left\langle\frac{dR}{d\theta}\right\rangle(e^+e^- \to W^+W^-)$ | `<dR/dtheta>(ee->WW)` | E = 205.92, thetamin = 0.4, thetamax = 0.6 |2.903 | 
| $\left\langle\frac{dR}{d\theta}\right\rangle(e^+e^- \to W^+W^-)$ | `<dR/dtheta>(ee->WW)` | E = 205.92, thetamin = 0.6, thetamax = 0.8 |4.445 | 
| $\left\langle\frac{dR}{d\theta}\right\rangle(e^+e^- \to W^+W^-)$ | `<dR/dtheta>(ee->WW)` | E = 205.92, thetamin = 0.8, thetamax = 1.0 |7.783 | 
